adding Itree denotation files

src/CoImp.v
@@ -252,7 +252,7 @@ Definition P:= <{X:=0; while X=0 do X:=X + 1 end }>.
 Definition stP:= X !-> 1.
 
 Lemma Return_interp_rtrn: forall {A} (x:A), (interp (Return x)) = rtrn x.
-Proof. intros. eval_ ((interp (Return x))). reflexivity. Qed.  
+Proof. intros. eval_ ((interp (Return x))). reflexivity. Qed.
 
   Theorem P_evals_to_stP: Eqp (interp (ceval_comp empty_st P)) (rtrn stP).
   Proof. 
@@ -323,3 +323,218 @@ match c with
           
 end.
 
+(* Implement constant folding for expressions and commands *)
+
+Fixpoint fold_constants_aexp (a : aexp) : aexp :=
+  match a with
+  | ANum n       => ANum n
+  | AId x        => AId x
+  | <{ a1 + a2 }>  =>
+    match (fold_constants_aexp a1,
+           fold_constants_aexp a2)
+    with
+    | (ANum n1, ANum n2) => ANum (n1 + n2)
+    | (a1', a2') => <{ a1' + a2' }>
+    end
+  | <{ a1 - a2 }> =>
+    match (fold_constants_aexp a1,
+           fold_constants_aexp a2)
+    with
+    | (ANum n1, ANum n2) => ANum (n1 - n2)
+    | (a1', a2') => <{ a1' - a2' }>
+    end
+  | <{ a1 * a2 }>  =>
+    match (fold_constants_aexp a1,
+           fold_constants_aexp a2)
+    with
+    | (ANum n1, ANum n2) => ANum (n1 * n2)
+    | (a1', a2') => <{ a1' * a2' }>
+    end
+  end.
+
+Example fold_aexp_ex1 :
+    fold_constants_aexp <{ (1 + 2) * X }>
+  = <{ 3 * X }>.
+Proof. reflexivity. Qed.
+
+(** Note that this version of constant folding doesn't do other
+    "obvious" things like eliminating trivial additions (e.g.,
+    rewriting [0 + X] to just [X]).: we are focusing attention on a
+    single optimization for the sake of simplicity.
+
+    It is not hard to incorporate other ways of simplifying
+    expressions -- the definitions and proofs just get longer.  We'll
+    consider optimizations in the exercises. *)
+
+Example fold_aexp_ex2 :
+  fold_constants_aexp <{ X - ((0 * 6) + Y) }> = <{ X - (0 + Y) }>.
+Proof. reflexivity. Qed.
+
+(** Not only can we lift [fold_constants_aexp] to [bexp]s (in the
+    [BEq], [BNeq], and [BLe] cases); we can also look for constant
+    _boolean_ expressions and evaluate them in-place as well. *)
+
+Fixpoint fold_constants_bexp (b : bexp) : bexp :=
+  match b with
+  | <{true}>        => <{true}>
+  | <{false}>       => <{false}>
+  | <{ a1 = a2 }>  =>
+      match (fold_constants_aexp a1,
+             fold_constants_aexp a2) with
+      | (ANum n1, ANum n2) =>
+          if n1 =? n2 then <{true}> else <{false}>
+      | (a1', a2') =>
+          <{ a1' = a2' }>
+      end
+  | <{ a1 <= a2 }>  =>
+      match (fold_constants_aexp a1,
+             fold_constants_aexp a2) with
+      | (ANum n1, ANum n2) =>
+          if n1 <=? n2 then <{true}> else <{false}>
+      | (a1', a2') =>
+          <{ a1' <= a2' }>
+      end
+
+  | <{ ~ b1 }>  =>
+      match (fold_constants_bexp b1) with
+      | <{true}> => <{false}>
+      | <{false}> => <{true}>
+      | b1' => <{ ~ b1' }>
+      end
+  | <{ b1 && b2 }>  =>
+      match (fold_constants_bexp b1,
+             fold_constants_bexp b2) with
+      | (<{true}>, <{true}>) => <{true}>
+      | (<{true}>, <{false}>) => <{false}>
+      | (<{false}>, <{true}>) => <{false}>
+      | (<{false}>, <{false}>) => <{false}>
+      | (b1', b2') => <{ b1' && b2' }>
+      end
+  end.
+
+Example fold_bexp_ex1 :
+  fold_constants_bexp <{ true && ~(false && true) }>
+  = <{ true }>.
+Proof. reflexivity. Qed.
+
+Example fold_bexp_ex2 :
+  fold_constants_bexp <{ (X = Y) && (0 = (2 - (1 + 1))) }>
+  = <{ (X = Y) && true }>.
+Proof. reflexivity. Qed.
+
+(** To fold constants in a command, we apply the appropriate folding
+    functions on all embedded expressions. *)
+
+Fixpoint fold_constants_com (c : com) : com :=
+  match c with
+  | <{ skip }> =>
+      <{ skip }>
+  | <{ x := a }> =>
+      <{ x := (fold_constants_aexp a) }>
+  | <{ c1 ; c2 }>  =>
+      <{ fold_constants_com c1 ; fold_constants_com c2 }>
+  | <{ if b then c1 else c2 end }> =>
+      match fold_constants_bexp b with
+      | <{true}>  => fold_constants_com c1
+      | <{false}> => fold_constants_com c2
+      | b' => <{ if b' then fold_constants_com c1
+                       else fold_constants_com c2 end}>
+      end
+  | <{ while b do c1 end }> =>
+      match fold_constants_bexp b with
+      | <{true}> => <{ while true do skip end }>
+      | <{false}> => <{ skip }>
+      | b' => <{ while b' do (fold_constants_com c1) end }>
+      end
+  end.
+
+Example fold_com_ex1 :
+  fold_constants_com
+    (* Original program: *)
+    <{ X := 4 + 5;
+       Y := X - 3;
+       if ((X - Y) = (2 + 4)) then skip
+       else Y := 0 end;
+       if (0 <= (4 - (2 + 1))) then Y := 0
+       else skip end;
+       while (Y = 0) do
+         X := X + 1
+       end }>
+  = (* After constant folding: *)
+    <{ X := 9;
+       Y := X - 3;
+       if ((X - Y) = 6) then skip
+       else Y := 0 end;
+       Y := 0;
+       while (Y = 0) do
+         X := X + 1
+       end }>.
+Proof. reflexivity. Qed.
+
+  Definition aequiv (a1 a2 : aexp) : Prop :=
+  forall (st : state),
+    aeval st a1 = aeval st a2.
+
+Definition bequiv (b1 b2 : bexp) : Prop :=
+  forall (st : state),
+    beval st b1 = beval st b2.
+  Definition atrans_sound (atrans : aexp -> aexp) : Prop :=
+    forall (a : aexp),
+      aequiv a (atrans a).
+  
+  Definition btrans_sound (btrans : bexp -> bexp) : Prop :=
+    forall (b : bexp),
+      bequiv b (btrans b).
+  
+      Theorem fold_constants_aexp_sound :
+      atrans_sound fold_constants_aexp.
+    Proof.
+      unfold atrans_sound. intros a. unfold aequiv. intros st.
+      induction a; simpl;
+        (* ANum and AId follow immediately *)
+        try reflexivity;
+        (* APlus, AMinus, and AMult follow from the IH
+           and the observation that
+                  aeval st (<{ a1 + a2 }>)
+                = ANum ((aeval st a1) + (aeval st a2))
+                = aeval st (ANum ((aeval st a1) + (aeval st a2)))
+           (and similarly for AMinus/minus and AMult/mult) *)
+        try (destruct (fold_constants_aexp a1);
+             destruct (fold_constants_aexp a2);
+             rewrite IHa1; rewrite IHa2; reflexivity). Qed.
+
+(*Theorem CSeq_congruence : forall c1 c1' c2 c2',
+             cequiv c1 c1' -> cequiv c2 c2' ->
+             cequiv <{ c1;c2 }> <{ c1';c2' }>.
+           Proof.
+             (* FILL IN HERE *) Admitted.*)
+
+
+Theorem equiv_while_true: forall b, bequiv b <{ true }> ->
+  forall c st,
+  Eqp (interp (ceval_comp st <{ while b do c end }>)) never.
+  Proof. intros. generalize dependent st .  generalize dependent c. cofix CIH.
+  intros. eval_ (interp (ceval_comp st <{ while b do c end }>)).
+  assert (beval st b = true). {apply H. } rewrite H0. eval_ (never).
+  constructor. 
+  eval_ (interp (st' <- ceval_comp st c; Step (ceval_comp st' <{ while b do c end }>))). destruct c.
+    + simpl. eval_ (interp (Step (ceval_comp st <{ while b do skip end }>))). eval_ (never).
+      eval_ (never). repeat constructor. apply CIH.
+    + simpl. eval_ (never). repeat constructor. 
+      eval_ (interp (Step (ceval_comp (t_update st x (aeval st a)) <{ while b do x := a end }>))). 
+      eval_ (never). repeat constructor. apply CIH. Admitted. 
+
+Theorem constant_folding_com: 
+forall c st, Eqp (interp (ceval_comp st c)) (interp (ceval_comp st (fold_constants_com c))).
+Proof. cofix CIH. intros. destruct c.
+  - simpl. eval_ (interp (ceval_comp st <{ skip }>)).
+  - simpl. eval_ (interp (ceval_comp st <{ x := a }>)). 
+    eval_ (interp (ceval_comp st <{ x := (fold_constants_aexp a) }>)).
+    rewrite fold_constants_aexp_sound. apply eqp_refl.
+  - eval_ (interp (ceval_comp st <{ c1; c2 }>)).
+    eval_ (interp (ceval_comp st <{ (fold_constants_com c1); (fold_constants_com c2) }>)). simpl. 
+     admit.
+  - admit.
+  - cofix CIH1. eval_ (interp (ceval_comp st <{ while b do c end }>)). 
+    destruct b eqn: Hb.
+    + simpl. eval_ (interp (ceval_comp st <{ while true do skip end }>)). constructor.  apply CIH1. 
